Improved list match primitive.

lib.v
@@ -213,24 +213,17 @@ Definition eq_list : val := rec: "loop" "eq" "l1" "l2" :=
      end
   end.
 
-Fixpoint list_match (vars : list string) (l : string) (k : expr) : expr :=
+Fixpoint list_match_aux (vars : list string) (l : expr) (k : expr) : expr :=
   match vars with
   | [] =>
-    match: l with SOME <> => NONEV | NONE => k end
-  | v :: vars =>
+    match: l with SOME <> => NONEV | NONE => k #() end
+  | var :: vars =>
+    let k' := if decide (var ∈ vars) then k else k (Fst var) in
     match: l with
-      SOME l =>
-      let: v := Fst l in
-      let: l := Snd l in
-      list_match vars l k
+      SOME var => list_match_aux vars (Snd var) k'
     | NONE => NONEV
     end
   end.
-
-Notation "'list_match:' vars := l 'in' e" :=
-  (list_match vars l e)%E
-  (at level 200, vars at level 1, l, e at level 200,
-  format "'[' 'list_match:'  vars  :=  '[' l ']'  'in'  '/' e ']'") : expr_scope.
 
 Definition insert_sorted : val := rec: "loop" "le" "x" "l" :=
   match: "l" with
@@ -269,37 +262,70 @@ Lemma substC x1 x2 v1 v2 e :
   subst x1 v1 (subst x2 v2 e) = subst x2 v2 (subst x1 v1 e).
 Proof. by move=> x12; elim: e => //= *; substC; congruence. Qed.
 
-Lemma subst_list_match_in var v vars l k :
-  var ∈ vars → l ∉ vars →
-  subst var v (list_match vars l k) = list_match vars l k.
+Lemma subst_list_match_aux var v vars el ek :
+  subst var v (list_match_aux vars el ek) =
+  list_match_aux vars (subst var v el) (
+    if decide (var ∈ vars) then ek else subst var v ek).
 Proof.
-elim: vars => [|var' vars IH]; first by set_solver.
-case: (decide (var = var')) => [<- _|ne].
-- rewrite elem_of_cons.
-  case/Decidable.not_or=> l_var l_fresh /=.
-  rewrite decide_False //.
-  rewrite decide_True; last by split; congruence.
-  rewrite decide_False //; by case; congruence.
-- rewrite !elem_of_cons; case => var_in; first congruence.
-  case/Decidable.not_or=> l_var' l_fresh /=.
-  rewrite decide_False; last congruence.
-  rewrite decide_True; last by split; congruence.
-  do 2![rewrite decide_True; last by split; congruence].
-  by rewrite IH.
+elim: vars => [|var' vars IH] //= in el ek *.
+case: (decide (var = var')) => [<-|ne].
+  rewrite decide_False; last by intuition congruence.
+  rewrite (@decide_True _ (var ∈ var :: vars)) //; last by set_solver.
+rewrite decide_True; last by intuition congruence.
+rewrite IH; case: (decide (var ∈ vars)) => [in_vars|nin_vars] /=.
+  rewrite (@decide_False _ (var = var')) //.
+  rewrite !(@decide_True  _ (var ∈ _)) //; set_solver.
+rewrite decide_False // (@decide_False _ (var ∈ _)); last by set_solver.
+case: decide => [in_vars'|nin_vars'] //=.
+by rewrite decide_False.
 Qed.
 
-Lemma subst_list_match var v vars l k :
-  var ∉ vars → l ≠ var → l ∉ vars →
-  subst var v (list_match vars l k) =
-  list_match vars l (subst var v k).
+Fixpoint close_vars (vars : list string) (k : expr) : expr :=
+  match vars with
+  | [] => λ: <>, k
+  | var :: vars =>
+    (if decide (var ∈ vars) then close_vars vars k
+     else λ: var, close_vars vars k)%E
+  end.
+
+Lemma subst_close_vars var v vars k :
+  var ∉ vars →
+  subst var v (close_vars vars k) = close_vars vars (subst var v k).
 Proof.
-move=> var_in var_l.
-elim: vars var_in => [|var' vars IH] /=; rewrite decide_False //.
-rewrite !elem_of_cons.
-case/Decidable.not_or => var_var' var_in.
-case/Decidable.not_or => l_var' l_vars.
-do ![rewrite decide_True; last by split; congruence].
-by rewrite IH.
+elim: vars => [|var' vars IH] //= in k *.
+case: decide => [in_vars'|nin_vars'] nin_vars /=.
+  apply: IH; set_solver.
+rewrite decide_True; last by split; eauto; set_solver.
+rewrite IH //; set_solver.
+Qed.
+
+Fact list_match_key : unit. Proof. exact: tt. Qed.
+
+Definition list_match :=
+  locked_with list_match_key (
+    λ vars l k,
+      list_match_aux vars l (close_vars vars k)
+  ).
+
+Canonical list_match_unlockable := [unlockable of list_match].
+
+Notation "'list_match:' vars := e1 'in' e2" :=
+  (list_match vars e1 e2)%E
+  (at level 200, vars at level 1, e1, e2 at level 200,
+  format "'[' 'list_match:'  vars  :=  '[' e1 ']'  'in'  '/' e2 ']'") : expr_scope.
+
+Lemma subst_list_match var v vars el ek :
+  subst var v (list_match vars el ek) =
+  list_match vars (subst var v el) (
+    if decide (var ∈ vars) then ek else subst var v ek).
+Proof.
+rewrite unlock subst_list_match_aux; case: decide => [//|nin_vars].
+congr list_match_aux; elim: vars => [|var' vars IH] //= in {el} ek nin_vars *.
+have neq : var ≠ var' by set_solver.
+have {}nin_vars : var ∉ vars by set_solver.
+case: (decide (var' ∈ vars)) => [in_vars'|nin_vars'] /=.
+  by rewrite IH.
+rewrite decide_True ?IH //; by intuition congruence.
 Qed.
 
 Definition binder_vars x : gset string :=
@@ -380,15 +406,25 @@ Ltac subst_free_vars_rem :=
     | H : context[_ ∈ ∅] |- _ => rewrite -> elem_of_empty in H
     | HQP : ¬ (?Q ∧ ?P), HP : ?P |- _ =>
       assert (¬ Q); [intros ?; apply HQP; by split|clear HQP]
+    | HQP : ¬ (?Q ∧ ?P) |- _ =>
+      rewrite -> not_and_l in HQP; destruct HQP
+    | H : ¬ ¬ _ |- _ => apply dec_stable in H
     | HP : ?P, HPQ : ?P -> ?Q |- _ => specialize (HPQ HP)
     | HNP : ¬ ?P, HP : ?P |- _ => destruct (HNP HP)
     | H : _ ∨ _ |- _ => destruct H
+    | e : ?x = _ |- context[?x] => rewrite e
     end
   ).
 
 Lemma subst_free_vars_rem var v e : var ∉ free_vars (subst var v e).
 Proof.
 by elim: e => /=; try by intros; subst_free_vars_rem; congruence.
+Qed.
+
+Lemma free_vars_subst var v e :
+  free_vars (subst var v e) = free_vars e ∖ {[var]}.
+Proof.
+elim: e => //=; intros; subst_free_vars_rem; subst; set_solver.
 Qed.
 
 Lemma subst_nsubst var v vars vs e :
@@ -409,6 +445,16 @@ Proof.
 elim: vars vs=> [|var' vars IH] [|v' vs]; try by rewrite ?elem_of_nil //=.
 rewrite elem_of_cons; case/Decidable.not_or => var_var' var_nin.
 by rewrite /= substC // IH.
+Qed.
+
+Lemma free_vars_nsubst vars vs e :
+  length vars = length vs →
+  free_vars (nsubst vars vs e) = free_vars e ∖ ⋃ (singleton <$> vars).
+Proof.
+elim: vars vs => [|var vars IH] [|v vs] //= in e *.
+  move=> _; set_solver.
+case=> e_len; rewrite free_vars_subst IH //.
+set_solver.
 Qed.
 
 Section ListLemmas.
@@ -459,30 +505,81 @@ Proof. by iIntros "?"; iApply twp_wp; iApply twp_cons. Qed.
 Definition list_to_expr :=
   foldr (fun (x : A) e => CONS (repr x) e) NILV.
 
-Lemma wp_list_match E vs vars (l : string) k Ψ :
-  l ∉ vars →
-  WP nsubst vars vs (subst l [] k) @ E {{ Ψ }} -∗
-  WP subst l (repr_list vs) (list_match vars l k) @ E {{ Ψ }}.
+Fixpoint napp (vars : list string) (vs : list val) :=
+  match vars, vs with
+  | var :: vars, v :: vs =>
+    if decide (var ∈ vars) then napp vars vs
+    else AppLCtx v :: napp vars vs
+  | [], [] => [AppLCtx #()]
+  | _, _ => []
+  end.
+
+Lemma wp_list_match_aux E (vs : list A) evs vars k Ψ :
+  elements (free_vars k) ## vars →
+  (∀ Ψ, Ψ (repr_list vs) -∗ WP evs @ E {{ Ψ }}) -∗
+  (if decide (length vars = length vs) then
+     WP fill (napp vars (map repr vs)) k @ E {{ Ψ }}
+   else Ψ NONEV) -∗
+  WP list_match_aux vars evs k @ E {{ Ψ }}.
 Proof.
 rewrite repr_list_eq.
-elim: vars vs k => [|var vars IH] [|v vs] k l_fresh /=.
-- by iIntros "post"; wp_pures; rewrite decide_True //=; wp_pures.
-- iIntros "post"; wp_pures; rewrite decide_True //= (lock (Val NONEV)).
-  by wp_pures.
-- iIntros "post"; wp_pures; rewrite decide_True //= {-2}(lock (Val NONEV)).
-  by wp_pures.
-- iIntros "post"; wp_pures; rewrite decide_True //=.
-  wp_pures; rewrite decide_False; last by case.
-  rewrite /= (@decide_True _ (l = l)) //.
-  move: l_fresh; rewrite elem_of_cons => /Decidable.not_or [l_var l_fresh].
-  rewrite decide_True; last by split => ?; congruence.
-  rewrite decide_False; last by case.
-  wp_pures.
-  rewrite decide_True; last by split=> ?; congruence.
-  case: (decide (var ∈ vars)) => [var_in|var_out].
-    rewrite subst_list_match_in // subst_nsubst //; by iApply IH.
-  rewrite subst_list_match // subst_nsubst_nin // substC //.
-  by iApply IH.
+elim: vars vs => [|var vars IH] [|v vs] /= in evs k *; iIntros (dis) "evs pS".
+- by wp_pures; wp_bind evs; iApply "evs"; wp_pures.
+- by wp_pures; wp_bind evs; iApply "evs"; wp_pures.
+- by wp_pures; wp_bind evs; iApply "evs"; wp_pures.
+rewrite /=; wp_pures; wp_bind evs; iApply "evs"; wp_pures.
+rewrite subst_list_match_aux /=.
+rewrite [if decide (var = var) then _ else _]decide_True //=.
+assert (fresh_var : var ∉ free_vars k) by set_solver.
+assert (dis' : elements (free_vars k) ## vars) by set_solver.
+iApply (IH with "[]"); try by iIntros (Ψ') "p'"; wp_pures; eauto.
+  case: decide => _ //=.
+  rewrite free_vars_subst decide_True //=.
+  set_solver.
+case: (decide (length vars = length vs)) => [eq_l|neq_l]; last first.
+  rewrite decide_False //; congruence.
+rewrite eq_l decide_True //.
+case: decide => [//|nin_vars] /=.
+rewrite decide_True //= subst_free_vars //.
+wp_pures; iApply wp_bind; wp_pures; by iApply wp_bind_inv.
+Qed.
+
+Lemma wp_close_vars E vars vs k Ψ :
+  length vars = length vs →
+  WP nsubst vars vs k @ E {{ Ψ }} -∗
+  WP fill (napp vars vs) (close_vars vars k) @ E {{ Ψ }}.
+Proof.
+elim: vars vs => [|var vars IH] [|v vs] //= in k Ψ *.
+  by iIntros (?) "p"; wp_pures.
+move=> [] e; iIntros "p".
+case: decide => [in_vars|nin_vars].
+  rewrite subst_free_vars; first by iApply IH.
+  rewrite free_vars_nsubst // elem_of_difference.
+  case => _; rewrite elem_of_union_list.
+  by apply; exists {[var]}; split; try set_solver.
+rewrite /=.
+iApply wp_bind.
+wp_pures.
+rewrite subst_nsubst_nin //.
+iApply wp_bind_inv.
+rewrite subst_close_vars //.
+by iApply IH.
+Qed.
+
+Lemma wp_list_match E vars (vs : list A) k Ψ :
+  (if decide (length vars = length vs) then
+     WP nsubst vars (map repr vs) k @ E {{ Ψ }}
+   else Ψ NONEV) -∗
+  WP list_match vars (repr vs) k @ E {{ Ψ }}.
+Proof.
+rewrite unlock; iIntros "post".
+assert (disj : elements (free_vars (close_vars vars k)) ## vars).
+  elim: vars => [|var vars IH] /= in k *; try case: decide => ?; set_solver.
+iApply (wp_list_match_aux E vs (repr vs)); eauto.
+  by iIntros (?) "?"; iApply wp_value.
+case: decide => ? //.
+iApply (wp_close_vars with "post").
+by rewrite map_length.
 Qed.
 
 Lemma twp_eq_list `{EqDecision A} (f : val) (l1 l2 : list A) Φ E :
